new version

T1-Stack/Stack.dfy
@@ -1,72 +1,198 @@
-class Stack{
-    var capacity : int; 
-    var list : array<int>; 
-    var top : int;
+class {:autocontracts} Stack
+{
+    ghost const maxLen: int;
+    ghost var data: seq<int>;
+
+    var arr: array<int>;
+    var max: int;
+    var head: int; //position
 
     predicate Valid()
-    reads this;
     {
-        capacity > 0 &&
-        capacity < list.Length &&
-        -1 <= top < capacity
+        max > 0 &&
+        arr.Length == max &&
+        maxLen == max &&
+        0 <= head <= max &&
+        data == arr[0..head]
     }
 
-    predicate Empty()
-    reads this;
+    constructor(n: int)
+    requires n > 0
+    ensures maxLen == n
+    ensures data == []
     {
-        top == -1
+        max := n;
+        arr := new int[n];
+        head := 0;
+
+        //spec
+        maxLen := n;
+        data := [];
     }
 
-    predicate Full()
-    reads this;
+    method Push(e: int) returns (b: bool)
+    ensures old(|data|) < maxLen ==> data == old(data) + [e]
+    ensures old(|data|) >= maxLen ==> data == old(data)
+    ensures b == (old(|data|) < maxLen)
+    ensures b == (|data| != old(|data|))
     {
-       top == capacity 
+        if head < max
+        {
+            arr[head] := e;
+            head := head + 1;
+
+            //spec
+            data := data + [e];
+
+            return true;
+        }
+        return false;
     }
 
-    constructor (c : int)
-    requires c > 0;
-    ensures Empty();
-    ensures fresh(list);
-    ensures this.list.Length == c;
-    ensures capacity == c && top == -1;
+    method Pop() returns (e: int)
+    requires |data|>0
+    ensures data == old(data)[0..old(|data|)-1]
+    ensures e == old(data)[|data|]
     {
-        capacity := c;
-        list := new int[c];
-        top := -1;
+        head := head - 1;
+        e := arr[head];
+
+        //spec
+        data := arr[0..head];
     }
 
-    method isEmpty() returns (r:bool)
-    requires Empty();
-    requires Valid();
-    ensures Empty();
+    method Drop()
+    ensures old(|data|)>0 ==> data == old(data)[0..old(|data|)-1]
     {
-        return true;
+        if head > 0
+        {
+            head := head -1;
+
+            //spec
+            data := arr[0..head];
+        }
     }
 
-    method isFull() returns (r:bool)
-    requires Full();
-    requires Valid();
-    ensures Full();
+    method Top() returns (e: int)
+    requires |data| > 0
+    ensures data == old(data)
+    ensures e == data[|data|-1]
     {
-        return true;
+        return arr[head-1];
     }
 
-    method Peek() returns (r:int)
-    requires Valid();
-    requires !Empty();
-    ensures list == old(list) && r == list[top]
+    method Full() returns (b: bool)
+    ensures b == (|data| == maxLen)
+    ensures data == old(data)
     {
-        return list[top];
+        return head == max;
     }
 
+    method Empty() returns (b: bool)
+    ensures b == (|data| == 0)
+    ensures data == old(data)
+    {
+        return head==0;
+    }
+
+    method Count() returns (n: int)
+    ensures n == |data|
+    ensures data == old(data)
+    {
+        n := head;
+    }
+
+    method Capacity() returns (s: int)
+    ensures s == maxLen
+    ensures data == old(data)
+    {
+        s := max;
+    }
+
+    method Reverse()
+    requires |data| > 0
+    ensures |data| == old(|data|)
+    ensures reversed(data, old(data))
+	ensures forall k :: 0 <= k < head ==> arr[k] == old(arr[head-1 - k]);
+    {
+
+        var i := 0;
+        var j := head-1;
+        while i < (j+1)/2
+        invariant 0 <= i <= (j+1)/2
+        invariant 0 <= j < head <= arr.Length;
+		invariant forall k :: 0 <= k < i || j-i < k <= j ==> arr[k] == old(arr[j-k]);
+		invariant forall k :: i <= k <= j-i ==> arr[k] == old(arr[k]);
+        {
+            arr[i], arr[j-i] := arr[j-i], arr[i];
+            i := i + 1;
+        }
+
+        data := arr[0..head];
+        
+    }
+}
+predicate permutacao (a:seq<int>, b:seq<int>)
+{
+    multiset(a) == multiset(b)
+}
+predicate reversed(sq1: seq<int>, sq2: seq<int>)
+requires |sq1| == |sq2|
+{
+    forall i :: 0 <= i < |sq1| ==> sq1[i] == sq2[|sq2|-1-i]
+}
+
+method Main()
+{
+    var s := []; 
+    var t := [];
+    assert reversed(s,t); //validate predicate for empty 
+    s := [1,2];
+    t := [2,1];
+    assert reversed(s,t); //validate predicate for not empty
+
+    var stack := new Stack(4);
+    var cap := stack.Capacity();
+    assert cap == 4; 
+
+    var empt := stack.Empty();
+    assert empt; 
+
+    var full := stack.Full();
+    assert !full;
+
+    var push := stack.Push(1);
+    assert push == true;
+    push := stack.Push(2);
+    assert push == true;
+    push := stack.Push(3);
+    assert push == true;
+    push := stack.Push(4);
+    assert push == true; //max = 4
+
+    push := stack.Push(5);
+    assert push == false; //should not push anymore
+
+    empt := stack.Empty();
+    assert !empt;
+
+    full := stack.Full();
+    assert full;
+
+    var count := stack.Count();
+    assert count == 4;
+
+    var top := stack.Top();
+    assert top == 4;
+    assert stack.data == [1,2,3,4];
     
-    //method Push (r:int)
-    //modifies list, `top;
-    //requires Valid();
-    //requires !Full();
-    //ensures r == list[top];
-    //{
-    //    top := top+1;
-    //    list[top] := r;
-    //}
+    stack.Reverse();
+    assert stack.data == [4,3,2,1];
+
+    stack.Drop();
+    assert stack.data == [4,3,2];
+
+    var pop := stack.Pop();
+    assert pop == 2;
+    
 }
